---
title: 通项已知，放缩差比
description: >
  通项已知，放缩差比
date: 2023-10-25
weight: 2


---

{{< alert >}}

放缩差比

{{< /alert >}}


{{< alert >}}This is an alert.{{< /alert >}}
{{< alert title="Note" >}}This is an alert with a title.{{< /alert >}}
{{% alert title="Note" %}}This is an alert with a title and **Markdown**.{{% /alert %}}
{{< alert color="success" >}}This is a successful alert.{{< /alert >}}
{{< alert color="warning" >}}This is a warning.{{< /alert >}}
{{< alert color="warning" title="Warning" >}}This is a warning with a title.{{< /alert >}}



【】证明：$\cfrac{2 \sqrt{2} - 1}{\sqrt{2} \cdot 2^2} +\cfrac{3 \sqrt{3} - 1}{\sqrt{3} \cdot 2^3} + \cdots +\cfrac{n \sqrt{n} - 1}{\sqrt{n} \cdot 2^n}< \cfrac{3}{2}$

【思路】通项分析：$\cfrac{n \sqrt{n} - 1}{\sqrt{n} \cdot 2^n} < \cfrac{n \sqrt{n}}{\sqrt{n} \cdot 2^n }= \cfrac{n}{2^n}$

$$ \sum_{i=2}^{i=n}\cfrac{i}{2^i} = \cfrac{3}{2} - \cfrac{n + 2}{2^{n+1}}$$

【解析】




























